Update deriv to use psg

nola/iris/deriv.v
@@ -1,177 +1,109 @@
 (** * Derivability *)
 
-From nola.util Require Export intp.
-From iris.bi Require Import lib.fixpoint.
+From nola.util Require Export intp psg.
+From nola.iris Require Export order.
+From iris.bi Require Import bi.
 From iris.proofmode Require Import proofmode.
 Import PintpNotation.
 
-(** ** Preliminaries *)
-
-(** [dwrap]: Wrapper for a derivability *)
-
-#[projections(primitive)]
-Record dwrap (A : Type) := Dwrap { dunwrap : A }.
-Arguments Dwrap {_} _.
-Arguments dunwrap {_} _.
-Add Printing Constructor dwrap.
-
-(** Notation for derivability *)
-Module DerivNotation.
-  Notation "⸨ J ⸩( δ )" := (dunwrap δ J) (format "⸨  '[' J  ']' ⸩( δ )").
-End DerivNotation.
-Import DerivNotation.
-
-(** Type for a derivability predicate *)
-Notation deriv JUD PROP := (dwrap (JUD → PROP)).
+(** ** Derivability *)
 
 (** [judg]: Judgment with the parameterized interpretation *)
 #[projections(primitive)]
 Structure judg (PROP : bi) : Type := Judg {
   judg_car :> Type;
   (** Interpretation parameterized over derivability candidates *)
-  #[canonical=no] judg_Pintp :: Pintp (deriv judg_car PROP) judg_car PROP;
+  #[canonical=no] judg_Pintp :: Pintp (judg_car → PROP) judg_car PROP;
 }.
 Arguments judg_car {PROP JUDG} : rename.
 Arguments judg_Pintp {PROP JUDG} : rename.
 
 Section deriv.
-  Context {PROP : bi} {JUDG : judg PROP}.
-  Implicit Type (J : JUDG) (δ : deriv JUDG PROP) (ih : deriv JUDG PROP → Prop).
-
-  (** Soundness of a derivability [δ] with respect to the semantics at [δ'] *)
-  Definition dsound δ δ' : PROP := ∀ J, ⸨ J ⸩(δ) -∗ ⟦ J ⟧(δ').
-  Definition dtrans δ δ' : PROP := ∀ J, ⸨ J ⸩(δ) -∗ ⸨ J ⸩(δ').
+  Context {PROP} {JUDG : judg PROP}.
+  Implicit Type (J : JUDG) (δ : JUDG → PROP) (ih : (JUDG → PROP) → Prop).
 
   (** ** [Deriv ih δ] : [δ] is a good derivability predicate
 
     [ih] is the inductive hypothesis, used for parameterized induction *)
-
-  Inductive Deriv ih δ : Prop := {
-    (** For [Deriv_intp] *)
-    Deriv_byintp' :
-      (* Parameterization by [Deriv'] is for strict positivity *)
-      ∃ Deriv' : _ → Prop, (∀ δ', Deriv' δ' → Deriv ih δ') ∧ ∀ J,
-        (∀ δ', ⌜Deriv' δ'⌝ → ⌜ih δ'⌝ →
-          □ dsound δ δ' -∗ □ dtrans δ δ' -∗ ⟦ J ⟧(δ')) -∗ ⸨ J ⸩(δ)
-  }.
+  Definition Deriv ih δ := Psgoidp (OT:=JUDG → PROP) pintp ih δ.
   Existing Class Deriv.
 
-  (** Get the derivability [⸨ J ⸩(δ)] by the interpretaion *)
-  Lemma Deriv_byintp `{!Deriv ih δ} {J} :
+  (** [Deriv] is monotone over the inductive hypothesis *)
+  Lemma Deriv_mono `{!Deriv ih δ} (ih' : _ → Prop) :
+    (∀ δ', ih δ' → ih' δ') → Deriv ih' δ.
+  Proof. move=> to. move: Deriv0. by apply Psgoidp_mono. Qed.
+
+  (** Parameterized induction principle for [Deriv] *)
+  Lemma Deriv_ind `{!Deriv ih' δ} ih :
+    Deriv (λ δ', ih δ' ∧ ih' δ') ⊑ ih → ih δ.
+  Proof. by apply Psgoidp_ind. Qed.
+
+  (** Get the derivability [δ J] by the interpretaion *)
+  Lemma to_Deriv `{!Deriv ih δ} {J} :
     ((* Take any good derivability predicate [δ'] *) ∀ δ', ⌜Deriv ih δ'⌝ →
       (* Can use the inductive hypothesis *) ⌜ih δ'⌝ →
-      (* Can turn [δ] into the semantics at [δ'] *)
-        □ dsound δ δ' -∗
-      (* Can turn [δ] into [δ'] *) □ dtrans δ δ' -∗
+      (* Can turn [δ] into the semantics at [δ'] *) ⌜∀ J, δ J ⊢ ⟦ J ⟧(δ')⌝ →
       (* The semantics at [δ'] *) ⟦ J ⟧(δ'))
-    -∗ (* The derivability at [δ] *) ⸨ J ⸩(δ).
+    ⊢ (* The derivability at [δ] *) δ J.
   Proof.
-    have X := Deriv_byintp' ih δ. move: X=> [dy[dyto byintp]]. iIntros "→".
-    iApply byintp. iIntros (δ' dyd'). apply dyto in dyd'. by iApply "→".
+    iIntros "to". iApply (to_Psgoidp Deriv0). iIntros (?[?[??]]).
+    by iApply "to".
   Qed.
-
-  (** [Deriv] is monotone over the inductive hypothesis *)
-  Lemma Deriv_mono `{D : !Deriv ih δ} (ih' : _ → Prop) :
-    (∀ δ', ih δ' → ih' δ') → Deriv ih' δ.
+  Lemma eqv_Deriv `{!Deriv ih δ} {J} :
+    δ J ⊣⊢ ∀ δ', ⌜Deriv ih δ'⌝ → ⌜ih δ'⌝ → ⌜∀ J, δ J ⊢ ⟦ J ⟧(δ')⌝ → ⟦ J ⟧(δ').
   Proof.
-    move=> ihto. move: δ D. fix FIX 2=> δ [[dy[dyto byintp]]]. split.
-    exists (Deriv ih'). split; [done|]=>/= ?. iIntros "big". iApply byintp.
-    iIntros (???). iApply "big"; iPureIntro; by [apply FIX, dyto|apply ihto].
-  Qed.
-
-  (** [Deriv] can accumulate the inductive hypothesis *)
-  Lemma Deriv_acc res {ih δ} :
-    (∀ δ', Deriv (λ δ', res δ' ∧ ih δ') δ' → res δ') → Deriv ih δ → res δ.
-  Proof.
-    move=> to dyd. apply to. move: δ dyd. fix FIX 2=> δ [[dy[dyto byintp]]].
-    split. exists (Deriv (λ δ, res δ ∧ ih δ)). split; [done|]=>/= ?.
-    iIntros "big". iApply byintp. iIntros (? dyd' ?). move: dyd'=>/dyto/FIX ?.
-    iApply "big"; iPureIntro; [done|]. split; by [apply to|].
-  Qed.
-
-  (** Introduce a derivability via semantics *)
-  Lemma Deriv_intro `{!Deriv ih δ} {J} :
-    (∀ δ', ⌜Deriv ih δ'⌝ → ⌜ih δ'⌝ → ⟦ J ⟧(δ')) ⊢ ⸨ J ⸩(δ).
-  Proof.
-    iIntros "∀". iApply Deriv_byintp. iIntros (???) "_ _". by iApply "∀".
+    iSplit; iIntros "?"; iStopProof; [|by exact to_Deriv]. iIntros "?" (????).
+    by iStopProof.
   Qed.
 
   (** Map derivabilities via semantics *)
   Lemma Deriv_map `{!Deriv ih δ} {J J'} :
     (∀ δ', ⌜Deriv ih δ'⌝ → ⌜ih δ'⌝ → ⟦ J ⟧(δ') -∗ ⟦ J' ⟧(δ')) -∗
-    ⸨ J ⸩(δ) -∗ ⸨ J' ⸩(δ).
+    δ J -∗ δ J'.
   Proof.
-    iIntros "∀ J". iApply Deriv_byintp. iIntros (???) "#→ _".
-    iApply "∀"; by [| |iApply "→"].
+    iIntros "∀ J". iApply to_Deriv. iIntros (??? to).
+    iApply "∀"; by [| |iApply to].
   Qed.
   Lemma Deriv_map2 `{!Deriv ih δ} {J J' J''} :
-    (∀ δ', ⌜Deriv ih δ'⌝ → ⌜ih δ'⌝ → ⟦ J ⟧(δ') -∗ ⟦ J' ⟧(δ') -∗
-      ⟦ J'' ⟧(δ')) -∗
-    ⸨ J ⸩(δ) -∗ ⸨ J' ⸩(δ) -∗ ⸨ J'' ⸩(δ).
+    (∀ δ', ⌜Deriv ih δ'⌝ → ⌜ih δ'⌝ → ⟦ J ⟧(δ') -∗ ⟦ J' ⟧(δ') -∗ ⟦ J'' ⟧(δ')) -∗
+    δ J -∗ δ J' -∗ δ J''.
   Proof.
-    iIntros "∀ J J'". iApply Deriv_byintp. iIntros (???) "#→ _".
-    iApply ("∀" with "[//] [//] [J]"); by iApply "→".
+    iIntros "∀ J J'". iApply to_Deriv. iIntros (??? to).
+    iApply ("∀" with "[//] [//] [J]"); by iApply to.
   Qed.
   Lemma Deriv_map3 `{!Deriv ih δ} {J J' J'' J'''} :
-    (∀ δ', ⌜Deriv ih δ'⌝ → ⌜ih δ'⌝ → ⟦ J ⟧(δ') -∗ ⟦ J' ⟧(δ') -∗
-      ⟦ J'' ⟧(δ') -∗ ⟦ J''' ⟧(δ')) -∗
-    ⸨ J ⸩(δ) -∗ ⸨ J' ⸩(δ) -∗ ⸨ J'' ⸩(δ) -∗ ⸨ J''' ⸩(δ).
+    (∀ δ', ⌜Deriv ih δ'⌝ → ⌜ih δ'⌝ → ⟦ J ⟧(δ') -∗ ⟦ J' ⟧(δ') -∗ ⟦ J'' ⟧(δ') -∗
+      ⟦ J''' ⟧(δ')) -∗
+    δ J -∗ δ J' -∗ δ J'' -∗ δ J'''.
   Proof.
-    iIntros "∀ J J' J''". iApply Deriv_byintp. iIntros (???) "#→ _".
-    iApply ("∀" with "[//] [//] [J] [J']"); by iApply "→".
+    iIntros "∀ J J' J''". iApply to_Deriv. iIntros (??? to).
+    iApply ("∀" with "[//] [//] [J] [J']"); by iApply to.
   Qed.
   Lemma Deriv_mapl `{!Deriv ih δ} {Js J'} :
     (∀ δ', ⌜Deriv ih δ'⌝ → ⌜ih δ'⌝ →
       ([∗ list] J ∈ Js, ⟦ J ⟧(δ')) -∗ ⟦ J' ⟧(δ')) -∗
-    ([∗ list] J ∈ Js, ⸨ J ⸩(δ)) -∗ ⸨ J' ⸩(δ).
+    ([∗ list] J ∈ Js, δ J) -∗ δ J'.
   Proof.
-    iIntros "∀ Js". iApply Deriv_byintp. iIntros (???) "#→ _".
-    iApply "∀"; [done..|]. iInduction Js as [|J Js] "IH"=>/=; [done|].
-    iDestruct "Js" as "[J Js]". iSplitL "J"; by [iApply "→"|iApply "IH"].
+    iIntros "∀ Js". iApply to_Deriv. iIntros (??? to). iApply "∀"; [done..|].
+    iStopProof. elim: Js; [done|]=>/= ?? IH. iIntros "[J ?]".
+    iSplitL "J"; by [iApply to|iApply IH].
   Qed.
 
   (** ** [der]: The best derivability predicate *)
-
-  (** [der_gen]: What becomes [der] by taking [bi_least_fixpoint] *)
-  Definition der_gen (self : JUDG → PROP) J : PROP :=
-    ∀ δ, ⌜Deriv (λ _, True) δ⌝ → □ dsound (Dwrap self) δ -∗
-      □ dtrans (Dwrap self) δ -∗ ⟦ J ⟧(δ).
-  #[export] Instance der_gen_mono : BiMonoPred (A:=leibnizO _) der_gen.
-  Proof.
-    split; [|solve_proper]=> Φ Ψ ??. iIntros "#ΦΨ" (?) "big".
-    iIntros (??) "#Ψδ #Ψδ'".
-    iApply "big"; [done|..]; iIntros "!> % ?"; [iApply "Ψδ"|iApply "Ψδ'"];
-      by iApply "ΦΨ".
-  Qed.
-
-  (** [der]: The best derivability predicate *)
-  Definition der_def : deriv JUDG PROP :=
-    Dwrap (bi_least_fixpoint (A:=leibnizO _) der_gen).
-  Lemma der_aux : seal (@der_def). Proof. by eexists. Qed.
-  Definition der := der_aux.(unseal).
-  Lemma der_unseal : der = der_def. Proof. exact: seal_eq. Qed.
+  Definition der : JUDG → PROP := psg (OT:=JUDG → PROP) pintp.
 
   (** [der] satisfies [Deriv] *)
   #[export] Instance der_Deriv : Deriv (λ _, True) der.
-  Proof.
-    rewrite der_unseal. split. eexists _. split; [done|]=>/=. iIntros (?) "big".
-    rewrite least_fixpoint_unfold. iIntros (??) "#→δ #→δ'".
-    iApply "big"; [done..| |]; iIntros "!> % ?/="; by [iApply "→δ"|iApply "→δ'"].
-  Qed.
+  Proof. apply Psgoidp_Psgoid, psg_Psgoid. Qed.
 
-  (** [der] is sound w.r.t. the interpretation under [der] *)
-  Lemma der_sound : ⊢ dsound der der.
-  Proof.
-    rewrite der_unseal. iApply (least_fixpoint_ind (A:=leibnizO _)).
-    iIntros "!> % gen". rewrite -der_unseal.
-    iApply ("gen" $! _ der_Deriv); iIntros "!> % /="; rewrite der_unseal.
-    { iIntros "[$ _]". } { iIntros "[_ $]". }
-  Qed.
+  (** [der] is sound w.r.t. the semantics at [der] *)
+  Lemma der_sound {J} : der J ⊢ ⟦ J ⟧(der).
+  Proof. move: J. exact (psg_post (OT:=JUDG → PROP)). Qed.
 End deriv.
 
 (** ** Derivability-parameterized interpretation *)
 Class Dintp (JUD : Type) (A : ofe) (PROP : bi) := DINTP {
-  dintp :: Pintp (deriv JUD PROP) A PROP;
+  dintp :: Pintp (JUD → PROP) A PROP;
   dintp_ne {δ} :: NonExpansive (dintp δ);
 }.
 Hint Mode Dintp - ! - : typeclass_instances.
