nola/iris/order.v
@@ -1,0 +1,34 @@
+(** * Order theory *)
+
+From nola.util Require Export order.
+From iris.bi Require Import bi.
+From iris.proofmode Require Import proofmode.
+
+Implicit Type PROP : bi.
+
+(** ** Pre-order for [PROP] *)
+Canonical Structure biPro PROP := Proty PROP (⊢) _.
+
+(** ** [biPro] has the meet and join *)
+#[export] Program Instance bin_meet_bi {PROP} : BinMeet PROP :=
+  BIN_MEET (∧)%I _ _ _.
+Next Obligation. move=> *. by iIntros "[? _]". Qed.
+Next Obligation. move=> *. by iIntros "[_ ?]". Qed.
+Next Obligation.
+  move=> > le le'. iIntros "?". iSplit; by [iApply le|iApply le'].
+Qed.
+#[export] Program Instance bin_join_bi {PROP} : BinJoin PROP :=
+  BIN_JOIN (∨)%I _ _ _.
+Next Obligation. move=> *. iIntros "?". by iLeft. Qed.
+Next Obligation. move=> *. iIntros "?". by iRight. Qed.
+Next Obligation.
+  move=> > le le'. iIntros "[?|?]"; by [iApply le|iApply le'].
+Qed.
+#[export] Program Instance big_meet_bi {PROP} : BigMeet PROP :=
+  BIG_MEET (λ _ S Φ, ∀ a, ⌜S a⌝ → Φ a)%I _ _.
+Next Obligation. move=> *. iIntros "to". by iApply "to". Qed.
+Next Obligation. move=> > to. iIntros "?" (??). iStopProof. by apply to. Qed.
+#[export] Program Instance big_join_bi {PROP} : BigJoin PROP :=
+  BIG_JOIN (λ _ S Φ, ∃ a, ⌜S a⌝ ∧ Φ a)%I _ _.
+Next Obligation. move=> *. iIntros "?". iExists _. by iSplit. Qed.
+Next Obligation. move=> > to. iIntros "[%[% ?]]". iStopProof. by apply to. Qed.
